KLR/Core/Basic.lean
@@ -92,22 +92,19 @@ inductive Stmt where
 @[serde tag = 105]
 structure Kernel where
   name : String
-  inputs : List TensorSram -- TODO change to TensorArg
-  outputs : List TensorSram -- TODO change to TensorArg
+  inputs : List TensorName
+  outputs : List TensorName
   body : List Stmt
   deriving BEq, FromCBOR, FromJson, FromSexp, Repr, ToCBOR, ToJson, ToSexp
 
 -- Utilities
 
 class Tensors (a : Type) where
-  tensors : a -> List TensorSram
+  tensors : a -> List TensorName
 export Tensors (tensors)
 
-instance : Tensors TensorSram where
+instance : Tensors TensorName where
   tensors tn := [tn]
-
-instance : Tensors TensorArg where
-  tensors | .sram t => [t] | _ => []
 
 -- TODO: not efficient
 instance [Tensors a] : Tensors (List a) where
@@ -133,6 +130,6 @@ instance : Tensors Stmt where
   | .store dst _ vs => tensors (tensors dst :: vs.map tensors)
   | .oper _ => [] -- TODO
 
-def Kernel.internal (k : Kernel) : List TensorSram :=
+def Kernel.internal (k : Kernel) : List TensorName :=
   let ts := (k.body.map tensors).flatten.eraseDups
   (ts.removeAll (tensors k.inputs)).removeAll (tensors k.outputs)
